Modifiers/Merge.dfy
@@ -1,0 +1,245 @@
+module Modifiers.Merge {
+  
+  import opened Circ
+  import opened Scuf
+  import opened MapFunction
+  import opened ConservedSubcircuit
+  import opened Subcircuit
+  import opened Utils
+  import opened Eval
+
+  predicate ScufMapsCanMerge(mp1: ScufMap, mp2: ScufMap)
+  {
+    && SeqsNoIntersection(mp1.inputs, mp2.inputs)
+    && SeqsNoIntersection(mp1.outputs, mp2.outputs)
+    && SeqsNoIntersection(mp1.inputs, mp2.outputs)
+    && SeqsNoIntersection(mp1.outputs, mp2.inputs)
+    && SeqsNoIntersection(mp1.state, mp2.state)
+    && SeqsNoIntersection(mp1.inputs, StateONPsSeq(mp2.state))
+    && SeqsNoIntersection(mp2.inputs, StateONPsSeq(mp1.state))
+    && SeqsNoIntersection(mp1.outputs, StateINPsSeq(mp2.state))
+    && SeqsNoIntersection(mp2.outputs, StateINPsSeq(mp1.state))
+  }
+
+  function MergeScufMaps(mp1: ScufMap, mp2: ScufMap): (mp: ScufMap)
+    requires mp1.Valid()
+    requires mp2.Valid()
+    requires ScufMapsCanMerge(mp1, mp2)
+    ensures mp.Valid()
+  {
+    var inputs := mp1.inputs + mp2.inputs;
+    var outputs := mp1.outputs + mp2.outputs;
+    var state := mp1.state + mp2.state;
+    assert Seq.HasNoDuplicates(inputs) by {
+      NoDuplicatesInConcat(mp1.inputs, mp2.inputs);
+    }
+    assert Seq.HasNoDuplicates(outputs) by {
+      NoDuplicatesInConcat(mp1.outputs, mp2.outputs);
+    }
+    assert Seq.HasNoDuplicates(state) by {
+      NoDuplicatesInConcat(mp1.state, mp2.state);
+    }
+    assert SeqsNoIntersection(inputs, outputs) by {
+      ConcatSeqsNoIntersection(mp1.inputs, mp2.inputs, mp1.outputs, mp2.outputs);
+    }
+    assert SeqsNoIntersection(inputs, StateONPsSeq(state)) by {
+      ConcatSeqsNoIntersection(mp1.inputs, mp2.inputs, StateONPsSeq(mp1.state), StateONPsSeq(mp2.state));
+      assert StateONPsSeq(state) == StateONPsSeq(mp1.state) + StateONPsSeq(mp2.state);
+    }
+    assert SeqsNoIntersection(outputs, StateINPsSeq(state)) by {
+      ConcatSeqsNoIntersection(mp1.outputs, mp2.outputs, StateINPsSeq(mp1.state), StateINPsSeq(mp2.state));
+      assert StateINPsSeq(state) == StateINPsSeq(mp1.state) + StateINPsSeq(mp2.state);
+    }
+    ScufMap(inputs, outputs, state)
+  }
+
+  function MergeSF(uf1: UpdateFunction, uf2: UpdateFunction, si: SI): (so: SO)
+    requires uf1.Valid()
+    requires uf2.Valid()
+    requires |si.inputs| == uf1.input_width + uf2.input_width
+    requires |si.state| == uf1.state_width + uf2.state_width
+    ensures |so.outputs| == uf1.output_width + uf2.output_width
+    ensures |so.state| == uf1.state_width + uf2.state_width
+  {
+    var si1 := SI(si.inputs[..uf1.input_width], si.state[..uf1.state_width]);
+    var si2 := SI(si.inputs[uf1.input_width..], si.state[uf1.state_width..]);
+    var so1 := uf1.sf(si1);
+    var so2 := uf1.sf(si2);
+    var so := SO(so1.outputs + so2.outputs, so1.state + so2.state);
+    so
+  }
+
+  function MergeUpdateFunctions(uf1: UpdateFunction, uf2: UpdateFunction): (uf: UpdateFunction)
+    requires uf1.Valid()
+    requires uf2.Valid()
+    ensures uf.Valid()
+  {
+    var input_width := uf1.input_width + uf2.input_width;
+    var output_width := uf1.output_width + uf2.output_width;
+    var state_width := uf1.state_width + uf2.state_width;
+    UpdateFunction(
+      input_width, output_width, state_width,
+      (si: SI) requires |si.inputs| == input_width && |si.state| == state_width => MergeSF(uf1, uf2, si)
+    )
+  }
+
+  lemma ScufsNoIntersectionMapsCanMerge(c: Circuit, s1: Scuf, s2: Scuf)
+    requires c.Valid()
+    requires s1.Valid(c)
+    requires s2.Valid(c)
+    requires s1.sc !! s2.sc
+    ensures ScufMapsCanMerge(s1.mp, s2.mp)
+  {
+  }
+
+  lemma IslandScufsAllInputsAdd(c: Circuit, s1: Scuf, s2:Scuf)
+    requires c.Valid()
+    requires s1.Valid(c)
+    requires s2.Valid(c)
+    requires s1.sc !! s2.sc
+    requires IsIsland(c, s1.sc)
+    requires IsIsland(c, s2.sc)
+    ensures
+      reveal ScValid();
+      AllInputs(c, s1.sc + s2.sc) == AllInputs(c, s1.sc) + AllInputs(c, s2.sc)
+  {
+  }
+
+  lemma MergeEvaluatesCorrectly(c: Circuit, s1: Scuf, s2: Scuf, np: NP, fi: FI)
+    requires c.Valid()
+    requires s1.Valid(c)
+    requires s2.Valid(c)
+    requires s1.sc !! s2.sc
+    requires IsIsland(c, s1.sc)
+    requires IsIsland(c, s2.sc)
+    requires np in s1.mp.outputs || np in s2.mp.outputs ||
+             np in StateINPs(s1.mp.state) || np in StateINPs(s2.mp.state)
+    requires FICircuitValid(c, fi)
+    ensures
+      var s := MergeScufsImpl(c, s1, s2);
+      Evaluate(c, np, fi) == EvalOk(MFLookup(s, fi, np))
+  {
+  }
+
+  function MergeScufsImpl(c: Circuit, s1: Scuf, s2: Scuf): (s: Scuf)
+    requires c.Valid()
+    requires s1.Valid(c)
+    requires s2.Valid(c)
+    requires s1.sc !! s2.sc
+    requires IsIsland(c, s1.sc)
+    requires IsIsland(c, s2.sc)
+  {
+    var sc := s1.sc + s2.sc;
+    assert ScufMapsCanMerge(s1.mp, s2.mp) by {
+      ScufsNoIntersectionMapsCanMerge(c, s1, s2);
+    }
+    var mp := MergeScufMaps(s1.mp, s2.mp);
+    var uf := MergeUpdateFunctions(s1.uf, s2.uf);
+    var s := Scuf(sc, mp, uf);
+    s
+  }
+
+  function MergeScufs(c: Circuit, s1: Scuf, s2: Scuf): (s: Scuf)
+    requires c.Valid()
+    requires s1.Valid(c)
+    requires s2.Valid(c)
+    requires s1.sc !! s2.sc
+    requires IsIsland(c, s1.sc)
+    requires IsIsland(c, s2.sc)
+    ensures s.Valid(c)
+  {
+    var s := MergeScufsImpl(c, s1, s2);
+    var mp := s.mp;
+    var uf := s.uf;
+    var sc := s.sc;
+    assert s.Valid(c) by {
+      assert s.MapValid() by {
+        assert mp.Valid();
+        assert mp.InSc(sc) by {
+          reveal NPsInSc();
+          reveal Seq.ToSet();
+        }
+        assert uf.Valid();
+        assert ScufMapUpdateFunctionConsistent(mp, uf);
+      }
+      assert ScValid(c, s.sc) by {
+        reveal ScValid();
+      }
+      assert s.SomewhatValid(c) by {
+        assert ScValid(c, sc);
+        reveal Seq.ToSet();
+        reveal AllONPs();
+        reveal ConnOutputs();
+        reveal ConnInputs();
+        reveal UnconnInputs();
+        reveal AllSeq();
+        reveal ScValid();
+        reveal Scuf.SomewhatValid();
+        assert (AllONPs(c, sc) >= Seq.ToSet(mp.outputs) >= ConnOutputs(c, sc)) by {
+          assert AllONPs(c, sc) == AllONPs(c, s1.sc) + AllONPs(c, s2.sc);
+          assert Seq.ToSet(mp.outputs) == Seq.ToSet(s1.mp.outputs) + Seq.ToSet(s2.mp.outputs);
+          assert ConnOutputs(c, sc) <= ConnOutputs(c, s1.sc) + ConnOutputs(c, s2.sc);
+          assert AllONPs(c, sc) >= Seq.ToSet(mp.outputs);
+          assert Seq.ToSet(mp.outputs) >= ConnOutputs(c, sc);
+        }
+        assert (Seq.ToSet(mp.inputs) == AllInputs(c, sc)) by {
+          assert Seq.ToSet(mp.inputs) == Seq.ToSet(s1.mp.inputs) + Seq.ToSet(s2.mp.inputs);
+          IslandScufsAllInputsAdd(c, s1, s2);
+          assert AllInputs(c, sc) == AllInputs(c, s1.sc) + AllInputs(c, s2.sc);
+        }
+        assert (Seq.ToSet(mp.state) == AllSeq(c, sc)) by {
+          assert Seq.ToSet(mp.state) == Seq.ToSet(s1.mp.state) + Seq.ToSet(s2.mp.state);
+          assert AllSeq(c, sc) == AllSeq(c, s1.sc) + AllSeq(c, s2.sc);
+        }
+      }
+      assert s.EvaluatesCorrectly(c) by {
+        reveal Seq.ToSet();
+        forall np | np in Seq.ToSet(s.mp.outputs) || np in StateINPs(s.mp.state)
+          ensures ONPValid(c, np) || INPValid(c, np)
+        {
+          ScufFInputsAreValid(c, s);
+          ScufFOutputsAreValid(c, s);
+        }
+        forall fi: FI | FIValid(fi, s.mp.inputs, s.mp.state)
+          ensures FICircuitValid(c, fi)
+          ensures forall np :: np in Seq.ToSet(s.mp.outputs) || np in StateINPs(s.mp.state) ==>
+            Evaluate(c, np, fi) == EvalOk(MFLookup(s, fi, np))
+        {
+          assert FICircuitValid(c, fi) by {ScufValidFiValidToFICircuitValid(c, s, fi);}
+          forall np | np in Seq.ToSet(s.mp.outputs) || np in StateINPs(s.mp.state)
+            ensures Evaluate(c, np, fi) == EvalOk(MFLookup(s, fi, np))
+          {
+            MergeEvaluatesCorrectly(c, s1, s2, np, fi);
+            assert Evaluate(c, np, fi) == EvalOk(MFLookup(s, fi, np));
+          }
+        }
+        reveal Scuf.EvaluatesCorrectly();
+      }
+    }
+    s
+  }
+
+  function MergeInserter(c: Circuit, z1: ScufInserter, z2: ScufInserter): (r: (Circuit, Scuf))
+    requires c.Valid()
+    requires z1.Valid()
+    requires z2.Valid()
+  {
+    var (new_c, s1, s2) := InsertTwo(c, z1, z2);
+    reveal DualInsertion();
+    var s := MergeScufs(new_c, s1, s2);
+    (new_c, s)
+  }
+
+  function MergeModifier(z1: ScufInserter, z2: ScufInserter): (r: ScufInserter)
+    requires z1.Valid()
+    requires z2.Valid()
+  {
+    reveal ScufInserter.Valid();
+    var uf := MergeUpdateFunctions(z1.uf, z2.uf);
+    ScufInserter(
+      uf,
+      (c: Circuit) requires c.Valid() => MergeInserter(c, z1, z2)
+    )
+  }
+
+}
