Modifiers/SelfConnect.dfy
@@ -1,0 +1,82 @@
+module Modifiers.Connect {
+
+  import opened Circ
+  import opened ConservedSubcircuit
+  import opened Scuf
+  import opened MapConnection
+  import opened MapFunction
+  import opened Eval
+  import opened Connection
+  import opened Utils
+  import opened Subcircuit
+  import opened SelfConnect
+
+  function {:vcs_split_on_every_assert} ConnectInserter(c: Circuit, z: ScufInserter, conn: InternalConnection): (r: (Circuit, Scuf))
+    requires c.Valid()
+    requires z.Valid()
+    requires conn.Valid()
+    requires InserterConnectionConsistent(z, conn)
+    ensures
+      var (new_c, new_s) := r;
+      && new_c.Valid()
+      && new_s.Valid(new_c)
+      && SimpleInsertion(c, new_c, new_s)
+  {
+    z.ValidForCircuit(c);
+    var (c1, s) := z.fn(c);
+    z.FnOutputsValid(c);
+    assert ScufConnectionConsistent(c1, s, conn) by {
+      reveal InserterConnectionConsistent();
+    }
+    assert MPConnectionConsistent(s.mp, conn) by {
+      reveal ScufConnectionConsistent();
+    }
+    //var connection := conn.GetConnection(s.mp);
+    //conn.GetConnectionProperties(c1, s);
+    //assert ConnectCircuitRequirements(c1, connection);
+    var (new_c, new_s) := ConnectCircuitScuf(c1, s, conn);
+    assert new_s.Valid(new_c) by {
+      assert new_s.MapValid();
+      assert new_s.SomewhatValid(new_c);
+      assert new_s.EvaluatesCorrectly(new_c) by {
+        //reveal ScValid();
+        //ScufFOutputsAreValid(c, this);
+        //reveal Seq.ToSet();
+        forall fi: FI | FIValid(fi, new_s.mp.inputs, new_s.mp.state) {
+          assert FICircuitValid(new_c, fi) by {ScufValidFiValidToFICircuitValid(new_c, new_s, fi);}
+          forall np | np in Seq.ToSet(new_s.mp.outputs) || np in StateINPs(new_s.mp.state) {
+            assert Evaluate(new_c, np, fi) == EvalOk(MFLookup(new_s, fi, np));
+          }
+        }
+      }
+    }
+    (new_c, new_s)
+  }
+
+  function ConnectModifier(z: ScufInserter, conn: InternalConnection): (new_z: ScufInserter)
+    requires z.Valid()
+    requires conn.Valid()
+    requires InserterConnectionConsistent(z, conn)
+    ensures new_z.Valid()
+  {
+    reveal ScufInserter.Valid();
+    reveal InserterConnectionConsistent();
+    var uf := ConnectUpdateFunction(z.uf, conn);
+    var new_z := ScufInserter(
+      uf,
+      (c: Circuit) requires c.Valid() => ConnectInserter(c, z, conn)
+    );
+    assert new_z.Valid() by {
+      assert new_z.uf.Valid();
+      forall c: Circuit | c.Valid()
+        ensures new_z.SpecificValid(c) 
+      {
+        assert new_z.fn.requires(c);
+        var (new_c, e) := new_z.fn(c);
+        assert (e.uf == new_z.uf);
+        assert SimpleInsertion(c, new_c, e);
+      }
+    }
+    new_z
+  }
+}
