Scuf.dfy
@@ -1,0 +1,435 @@
+module Scuf {
+
+  import Std.Collections.Seq
+  import opened Subcircuit
+  import opened Circ
+  import opened Eval
+  import opened Utils
+  import opened MapFunction
+
+  datatype Scuf = Scuf(
+    sc: set<CNode>,
+    mp: ScufMap,
+    uf: UpdateFunction
+  ) {
+
+    ghost predicate MapValid() {
+      && mp.Valid()
+      && mp.InSc(sc)
+      && uf.Valid()
+      && ScufMapUpdateFunctionConsistent(mp, uf)
+    }
+
+    opaque predicate SomewhatValid(c: Circuit)
+      requires c.Valid()
+    {
+      && ScValid(c, sc)
+      && (AllONPs(c, sc) >= Seq.ToSet(mp.outputs) >= ConnOutputs(c, sc))
+      && (Seq.ToSet(mp.state) == AllSeq(c, sc))
+      && (Seq.ToSet(mp.inputs) == AllInputs(c, sc))
+    }
+
+    opaque predicate SomewhatValidRelaxInputs(c: Circuit)
+      requires c.Valid()
+    {
+      && ScValid(c, sc)
+      && (AllONPs(c, sc) >= Seq.ToSet(mp.outputs) >= ConnOutputs(c, sc))
+      && (Seq.ToSet(mp.state) == AllSeq(c, sc))
+      // We relax the constraint on inputs a bit.
+      // This is useful if we've connected an input but still want to
+      // work with properties of the scuf.
+      && (AllINPs(c, sc) >= Seq.ToSet(mp.inputs) >= AllInputs(c, sc))
+    }
+
+    lemma SomewhatValidToRelaxInputs(c: Circuit)
+      requires c.Valid()
+      requires SomewhatValid(c)
+      ensures SomewhatValidRelaxInputs(c)
+    {
+      reveal SomewhatValid();
+      reveal SomewhatValidRelaxInputs();
+      reveal ConnInputs();
+      reveal UnconnInputs();
+      reveal Seq.ToSet();
+      assert AllInputs(c, sc) <= AllINPs(c, sc) by {
+        reveal AllINPs();
+        reveal NPsInSc();
+        reveal INPsValid();
+      }
+    }
+
+    ghost opaque predicate EvaluatesCorrectly(c: Circuit)
+      requires c.Valid()
+      requires ScValid(c, sc)
+      requires MapValid()
+      requires SomewhatValidRelaxInputs(c)
+    {
+      reveal ScValid();
+      ScufFOutputsAreValid(c, this);
+      reveal Seq.ToSet();
+      forall fi: FI :: FIValid(fi, mp.inputs, mp.state) ==>
+        assert FICircuitValid(c, fi) by {ScufValidFiValidToFICircuitValid(c, this, fi);}
+        forall np :: np in Seq.ToSet(mp.outputs) || np in StateINPs(mp.state) ==>
+          Evaluate(c, np, fi) == EvalOk(MFLookup(this, fi, np))
+    }
+
+    ghost predicate Valid(c: Circuit)
+      requires c.Valid()
+    {
+      && MapValid()
+      && ScValid(c, sc)
+      && SomewhatValid(c)
+      && assert SomewhatValidRelaxInputs(c) by {
+           SomewhatValidToRelaxInputs(c);
+         }
+      && EvaluatesCorrectly(c)
+    }
+
+    ghost predicate ValidRelaxInputs(c: Circuit)
+      requires c.Valid()
+    {
+      && MapValid()
+      && ScValid(c, sc)
+      && SomewhatValidRelaxInputs(c)
+      && EvaluatesCorrectly(c)
+    }
+
+    function f(fi: FI): (fo: FO)
+      requires MapValid()
+      requires FIValid(fi, mp.inputs, mp.state)
+      ensures FOValid(fo, mp.outputs, mp.state)
+    {
+      reveal UpdateFunction.Valid();
+      var si := mp.fi2si(fi);
+      var so := uf.sf(si);
+      var fo := mp.so2fo(so);
+      fo
+    }
+
+    lemma MapNPsInSc()
+      requires MapValid()
+      ensures NPsInSc(sc, mp.NPs())
+    {
+      reveal NPsInSc();
+      reveal Seq.ToSet();
+    }
+  }
+
+  lemma ScufFInputsAreValid(c: Circuit, e: Scuf)
+    requires c.Valid()
+    requires e.SomewhatValidRelaxInputs(c)
+    ensures forall np :: np in e.mp.inputs ==> INPValid(c, np)
+    ensures forall np :: np in StateONPs(e.mp.state) ==> ONPValid(c, np)
+  {
+    reveal Scuf.SomewhatValidRelaxInputs();
+    reveal AllSeq();
+    reveal INPsValid();
+    assert INPsValid(c, AllInputs(c, e.sc));
+    assert INPsValid(c, Seq.ToSet(e.mp.inputs));
+    reveal Seq.ToSet();
+    forall np | np in StateONPs(e.mp.state)
+      ensures ONPValid(c, np)
+    {
+      assert np.n in e.mp.state;
+      assert np.p == OUTPUT_0;
+      assert np.n in AllSeq(c, e.sc);
+      reveal ScValid();
+      assert np.n in c.NodeKind;
+    }
+  }
+
+  lemma ScufFOutputsAreValid(c: Circuit, e: Scuf)
+    requires c.Valid()
+    requires e.SomewhatValidRelaxInputs(c)
+    ensures forall np :: np in e.mp.outputs ==> ONPValid(c, np)
+    ensures forall np :: np in StateINPs(e.mp.state) ==> INPValid(c, np)
+  {
+    reveal ScValid();
+    reveal Scuf.SomewhatValidRelaxInputs();
+    reveal ONPsValid();
+    assert Seq.ToSet(e.mp.outputs) <= AllONPs(c, e.sc);
+    reveal Seq.ToSet();
+    reveal ONPsValid();
+    reveal AllSeq();
+    forall np | np in StateINPs(e.mp.state)
+      ensures INPValid(c, np)
+    {
+      assert np.n in AllSeq(c, e.sc);
+    }
+  }
+
+
+  ghost opaque predicate ScufSeqEvaluatesCorrectly(c: Circuit, e: Scuf)
+    requires c.Valid()
+    requires ScValid(c, e.sc)
+    requires e.MapValid()
+    requires e.SomewhatValidRelaxInputs(c)
+  {
+    reveal ScValid();
+    ScufFOutputsAreValid(c, e);
+    reveal Seq.ToSet();
+    forall fi: FI :: FIValid(fi, e.mp.inputs, e.mp.state) ==>
+      assert FICircuitValid(c, fi) by {ScufValidFiValidToFICircuitValid(c, e, fi);}
+      forall np :: np in Seq.ToSet(e.mp.outputs) || np in StateINPs(e.mp.state) ==>
+        Evaluate(c, np, fi) == EvalOk(MFLookup(e, fi, np))
+  }
+
+  lemma FInputsInSc(c: Circuit, e: Scuf)
+    requires c.Valid()
+    requires e.SomewhatValid(c)
+    ensures NPsInSc(e.sc, Seq.ToSet(e.mp.inputs))
+    ensures NPsInSc(e.sc, StateONPs(e.mp.state))
+  {
+    reveal Scuf.SomewhatValid();
+    reveal AllINPs();
+    reveal NPsInSc();
+    reveal Seq.ToSet();
+    reveal AllSeq();
+  }
+
+  lemma FOutputsInSc(c: Circuit, e: Scuf)
+    requires c.Valid()
+    requires e.SomewhatValid(c)
+    ensures NPsInSc(e.sc, Seq.ToSet(e.mp.outputs))
+    ensures NPsInSc(e.sc, StateINPs(e.mp.state))
+  {
+    reveal NPsInSc();
+    reveal Scuf.SomewhatValid();
+    reveal AllSeq();
+    reveal Seq.ToSet();
+    assert AllONPs(c, e.sc) >= Seq.ToSet(e.mp.outputs);
+  }
+
+  lemma FAllInSc(c: Circuit, e: Scuf)
+    requires c.Valid()
+    requires e.SomewhatValid(c)
+    ensures NPsInSc(e.sc, e.mp.NPs())
+  {
+    FInputsInSc(c, e);
+    FOutputsInSc(c, e);
+    reveal NPsInSc();
+  }
+
+  lemma StateInSc(c: Circuit, e: Scuf)
+    requires c.Valid()
+    requires e.SomewhatValid(c)
+    ensures Seq.ToSet(e.mp.state) <= e.sc
+  {
+    reveal Scuf.SomewhatValid();
+  }
+
+  lemma StaysInSc(c: Circuit, e: Scuf, np: NP)
+    requires c.Valid()
+    requires e.SomewhatValid(c)
+    requires INPValid(c, np)
+    requires np.n in e.sc
+    requires np !in e.mp.inputs
+    ensures np in c.PortSource
+    ensures c.PortSource[np].n in e.sc
+  {
+    reveal Circuit.Valid();
+    reveal Scuf.SomewhatValid();
+    reveal UnconnInputs();
+    reveal ConnInputs();
+    reveal Seq.ToSet();
+    assert np !in AllInputs(c, e.sc);
+  }
+
+  predicate OutputsInFOutputs(c: Circuit, e: Scuf)
+    requires c.Valid()
+  {
+    Seq.ToSet(e.mp.outputs) >= ConnOutputs(c, e.sc)
+  }
+
+  lemma InputsOfIslandNotInPortSource(c: Circuit, e: Scuf)
+    requires c.Valid()
+    requires IsIsland(c, e.sc)
+    requires e.Valid(c)
+    ensures SetsNoIntersection(Seq.ToSet(e.mp.inputs), c.PortSource.Keys)
+  {
+    reveal Seq.ToSet();
+    forall np | np in e.mp.inputs
+      ensures np !in c.PortSource
+    {
+      NPInFInputsOfIslandNotInPortSource(c, e, np);
+    }
+    assert forall np :: np in Seq.ToSet(e.mp.inputs) ==> np in e.mp.inputs;
+  }
+
+  lemma NPInFInputsOfIslandNotInPortSource(c: Circuit, e: Scuf, np: NP) 
+    requires c.Valid()
+    requires IsIsland(c, e.sc)
+    requires e.Valid(c)
+    requires np in e.mp.inputs
+    ensures np !in c.PortSource
+  {
+    reveal Seq.ToSet();
+    assert np in AllInputs(c, e.sc) by {
+      reveal Scuf.SomewhatValid();
+    }
+    assert |ConnInputs(c, e.sc)| == 0 by {
+      IsIslandNoInputs(c, e.sc);
+    }
+    assert np in UnconnInputs(c, e.sc) || np in SeqInputs(c, e.sc);
+    if np in UnconnInputs(c, e.sc) {
+      assert np !in c.PortSource by {
+        reveal UnconnInputs();
+      }
+    }
+    if np in SeqInputs(c, e.sc) {
+      reveal ONPsValid();
+      assert ONPValid(c, np) by {
+        reveal SeqInputs();
+      }
+    }
+  }
+
+  lemma ScufValidFiValidToFICircuitValid(c: Circuit, e: Scuf, fi: FI)
+    requires c.Valid()
+    requires e.SomewhatValidRelaxInputs(c)
+    requires FIValid(fi, e.mp.inputs, e.mp.state)
+    ensures FICircuitValid(c, fi)
+  {
+    reveal Scuf.SomewhatValidRelaxInputs();
+    assert Seq.ToSet(e.mp.inputs) >= AllInputs(c, e.sc);
+    assert Seq.ToSet(e.mp.inputs) == fi.inputs.Keys;
+    reveal ConnInputs();
+    reveal UnconnInputs();
+    reveal INPsValid();
+    assert fi.state.Keys == Seq.ToSet(e.mp.state);
+    assert fi.state.Keys == AllSeq(c, e.sc);
+    reveal AllSeq();
+    reveal ONPsValid();
+    reveal ScValid();
+    assert (forall np :: np in fi.inputs.Keys ==> INPValid(c, np));
+    assert (forall n :: n in fi.state.Keys ==> c.NodeKind[n].CSeq?);
+    reveal FICircuitValid();
+  }
+
+  lemma EntitiesSeparate(c: Circuit, e1: Scuf, e2: Scuf)
+    requires c.Valid()
+    requires e1.SomewhatValid(c)
+    requires e2.SomewhatValid(c)
+    requires e1.sc !! e2.sc
+    ensures e1.mp.NPs() !! e2.mp.NPs()
+  {
+    FAllInSc(c, e1);
+    FAllInSc(c, e2);
+    forall np | np in e1.mp.NPs()
+      ensures np !in e2.mp.NPs()
+    {
+      if np in e2.mp.NPs() {
+        reveal NPsInSc();
+        assert np.n in e1.sc;
+        assert np.n in e2.sc;
+        assert np.n in e1.sc * e2.sc;
+        assert false;
+      }
+    }
+  }
+
+  function ScufSwapUF(c: Circuit, e: Scuf, uf: UpdateFunction): (r: Scuf)
+    requires c.Valid()
+    requires e.Valid(c)
+    requires uf.Valid()
+    requires UpdateFunctionsEquiv(e.uf, uf)
+    ensures r.Valid(c)
+  {
+    var r := Scuf(e.sc, e.mp, uf);
+    assert r.SomewhatValid(c) by {
+      reveal Scuf.SomewhatValid();
+    }
+    r.SomewhatValidToRelaxInputs(c);
+    assert r.MapValid() by {
+      UFConsistentEquiv(e.uf, uf, e.mp);
+    }
+    assert ScValid(c, r.sc);
+    assert r.EvaluatesCorrectly(c) by {
+      reveal Scuf.EvaluatesCorrectly();
+      reveal UpdateFunctionsEquiv();
+    }
+    r
+  }
+
+  const NullScuf := Scuf({}, NullScufMap, NullUpdateFunction)
+
+  lemma NullScufValid(c: Circuit)
+    requires c.Valid()
+    ensures NullScuf.Valid(c)
+  {
+    var e := NullScuf;
+    assert ScValid(c, e.sc) by {
+      reveal ScValid();
+    }
+    assert e.uf.Valid() by {
+      NullUpdateFunctionValid();
+    }
+    assert e.MapValid() by {
+      NullScufMapValid();
+      reveal NPsInSc();
+      reveal Seq.ToSet();
+    }
+    assert e.SomewhatValid(c) by {
+      reveal AllONPs();
+      reveal Seq.ToSet();
+      reveal ConnOutputs();
+      reveal ConnInputs();
+      reveal UnconnInputs();
+      reveal Scuf.SomewhatValid();
+    }
+    e.SomewhatValidToRelaxInputs(c);
+    assert e.EvaluatesCorrectly(c) by {
+      reveal Seq.ToSet();
+      assert |Seq.ToSet(e.mp.outputs)| == 0;
+      assert |StateINPs(e.mp.state)| == 0;
+      reveal Scuf.EvaluatesCorrectly();
+    }
+    reveal Scuf.SomewhatValid();
+  }
+
+  function MFLookup(scuf: Scuf, fi: FI, np: NP): bool
+    requires scuf.MapValid()
+    requires FIValid(fi, scuf.mp.inputs, scuf.mp.state)
+    requires np in scuf.mp.outputs || np in StateINPs(scuf.mp.state)
+  {
+    assert !((np in scuf.mp.outputs) && (np in StateINPs(scuf.mp.state))) by {
+      reveal Seq.ToSet();
+      StateINPsSeqSame(scuf.mp.state);
+    }
+    if (np in scuf.mp.outputs) then
+      MFLookupOutput(scuf, fi, np)
+    else
+      MFLookupState(scuf, fi, np)
+  }
+
+  function MFLookupOutput(scuf: Scuf, fi: FI, np: NP): bool
+    requires scuf.MapValid()
+    requires FIValid(fi, scuf.mp.inputs, scuf.mp.state)
+    requires np in scuf.mp.outputs
+  {
+    var si := scuf.mp.fi2si(fi);
+    reveal UpdateFunction.Valid();
+    var so := scuf.uf.sf(si);
+    var fo := scuf.mp.so2fo(so);
+    assert FOValid(fo, scuf.mp.outputs, scuf.mp.state);
+    reveal Seq.ToSet();
+    fo.outputs[np]
+  }
+
+  function MFLookupState(scuf: Scuf, fi: FI, np: NP): bool
+    requires scuf.MapValid()
+    requires FIValid(fi, scuf.mp.inputs, scuf.mp.state)
+    requires np in StateINPs(scuf.mp.state)
+  {
+    reveal UpdateFunction.Valid();
+    var si := scuf.mp.fi2si(fi);
+    var so := scuf.uf.sf(si);
+    var fo := scuf.mp.so2fo(so);
+    assert FOValid(fo, scuf.mp.outputs, scuf.mp.state);
+    reveal Seq.ToSet();
+    fo.state[np.n]
+  }
+
+
+
+}
