SelfConnect.dfy
@@ -1,0 +1,526 @@
+module SelfConnect {
+
+  import opened Circ
+  import opened ConservedSubcircuit
+  import opened Scuf
+  import opened MapConnection
+  import opened MapFunction
+  import opened Eval
+  import opened Connection
+  import opened Utils
+  import opened Subcircuit
+
+  // A scuf is modified such that some of its outputs are connected to the inputs.
+  // The outputs remain unchanged, but the new input width is reduced.
+  // `InternalConnection` defines a mapping from the (new_inputs, outputs) to the original inputs.
+  datatype InternalConnection = InternalConnection(
+    ni_width: nat,  // Width of the new inputs
+    i_width: nat,   // Width of the original inputs
+    o_width: nat,   // Width of the outputs.
+    connections: map<nat, nat>, // Maps input indices to output indices
+    i2ni: seq<nat>, // A map that can be used to generate new_inputs from inputs.
+    nio2i: seq<(bool, nat)> // A map to generate inputs from new_inputs and outputs.
+  ) {
+    ghost opaque predicate Valid() {
+      && (ni_width <= i_width)
+      && (i_width <= ni_width + o_width)
+      && (|i2ni| == ni_width)
+      && (|nio2i| == i_width)
+      && Seq.HasNoDuplicates(i2ni)
+      && Seq.HasNoDuplicates(nio2i)
+      && (forall index: nat :: index in connections.Values ==> index < o_width)
+      && (forall index: nat :: index in connections.Keys ==> index < i_width)
+      && (forall ni_index: nat :: ni_index < ni_width ==> (
+        var i_index: nat := i2ni[ni_index];
+        && (i_index < i_width)
+        && var (from_output, index) := nio2i[i_index];
+        && (!from_output)
+        && (index == ni_index)
+      ))
+      && (forall i_index: nat :: i_index < i_width ==> (
+        var (from_output, index) := nio2i[i_index];
+        && ((!from_output) ==> index < ni_width && i2ni[index] == i_index && (i_index !in connections))
+        && ((from_output) ==> index < o_width && (i_index in connections) && (index == connections[i_index]))
+      ))
+    }
+    function NIO2I<T>(bni: seq<T>, bo: seq<T>): (bi: seq<T>)
+      requires Valid()
+      requires |bni| == ni_width
+      requires |bo| == o_width
+      ensures |bi| == i_width
+    {
+      reveal Valid();
+      seq(i_width, (i_index: int) requires 0 <= i_index < i_width =>
+        var (from_output, index) := nio2i[i_index];
+        if !from_output then
+          bni[index]
+        else
+          bo[index]
+      )
+    }
+
+    function I2NI<T>(bi: seq<T>): (bni: seq<T>)
+      requires Valid()
+      requires |bi| == i_width
+      ensures |bni| == ni_width
+    {
+      reveal Valid();
+      seq(ni_width, (ni_index: int) requires 0 <= ni_index < ni_width =>
+        var i_index := i2ni[ni_index];
+        assert i_index < i_width;
+        bi[i_index])
+    }
+
+    function MapConnectedInputs<T(==)>(bi: seq<T>): (r: set<T>)
+      requires Valid()
+      requires |bi| == i_width
+    {
+      reveal Valid();
+      (set index | index in connections :: bi[index])
+    }
+
+    lemma I2NIProperties<T>(bi: seq<T>)
+      requires Valid()
+      requires |bi| == i_width
+      requires Seq.HasNoDuplicates(bi)
+      ensures
+        var bni := I2NI(bi);
+        reveal Valid();
+        && Seq.HasNoDuplicates(bni)
+        && Seq.ToSet(bni) == Seq.ToSet(bi) - MapConnectedInputs(bi)
+    {
+      reveal Valid();
+      reveal Seq.ToSet();
+      reveal Seq.HasNoDuplicates();
+      var bni := I2NI(bi);
+      forall i_index: nat | i_index < i_width
+        ensures bi[i_index] in Seq.ToSet(bni) || bi[i_index] in MapConnectedInputs(bi)
+      {
+        var (from_output, index) := nio2i[i_index];
+        if from_output {
+          assert bi[i_index] in MapConnectedInputs(bi);
+        } else {
+          reveal Seq.ToSet();
+          assert bi[i_index] == bni[index];
+          assert bi[i_index] in Seq.ToSet(bni);
+        }
+      }
+    }
+
+    lemma NIO2I2NI<T>(bni: seq<T>, bo: seq<T>)
+      requires Valid()
+      requires |bni| == ni_width
+      requires |bo| == o_width
+      ensures I2NI(NIO2I(bni, bo)) == bni
+    {
+      reveal Valid();
+    }
+
+    function GetConnectedInputs(mp: ScufMap): (r: set<NP>)
+      requires Valid()
+      requires MPConnectionConsistent(mp, this)
+      ensures r <= Seq.ToSet(mp.inputs)
+    {
+      reveal Valid();
+      reveal Seq.ToSet();
+      (set i_index | i_index in connections :: mp.inputs[i_index])
+    }
+
+    function GetConnectedOutputs(mp: ScufMap): (r: set<NP>)
+      requires Valid()
+      requires MPConnectionConsistent(mp, this)
+      ensures r <= Seq.ToSet(mp.outputs)
+    {
+      reveal Valid();
+      reveal Seq.ToSet();
+      (set o_index | o_index in connections.Values :: mp.outputs[o_index])
+    }
+
+    lemma GetConnectionProperties(c: Circuit, s: Scuf)
+      requires Valid()
+      requires c.Valid()
+      requires s.Valid(c)
+      requires ScufConnectionConsistent(c, s, this)
+      ensures
+        reveal ScufConnectionConsistent();
+        var r := GetConnection(s.mp);
+        && (forall onp :: onp in r.Values ==> ONPValid(c, onp))
+        && (forall inp :: inp in r ==> INPValid(c, inp))
+        && (forall inp :: inp in r ==> NoPathInScuf(c, s, r[inp], inp))
+        && MPConnectionConsistent(s.mp, this)
+        && (r.Keys == GetConnectedInputs(s.mp))
+        && (r.Values == GetConnectedOutputs(s.mp))
+        && ConnectCircuitRequirements(c, r)
+    {
+      reveal ScufConnectionConsistent();
+      var np_connections := GetConnection(s.mp);
+      reveal Seq.ToSet();
+      s.SomewhatValidToRelaxInputs(c);
+      ScufFInputsAreValid(c, s);
+      ScufFOutputsAreValid(c, s);
+      assert ConnectCircuitRequirements(c, np_connections) by {
+        reveal ConnectCircuitRequirements();
+      }
+    }
+
+    function GetConnection(mp: ScufMap): (r: map<NP, NP>)
+      requires Valid()
+      requires mp.Valid()
+      requires MPConnectionConsistent(mp, this)
+      ensures MPConnectionConsistent(mp, this)
+      ensures r.Keys == GetConnectedInputs(mp)
+      ensures r.Values == GetConnectedOutputs(mp)
+    {
+      reveal Valid();
+      assert |mp.inputs| == i_width;
+      assert (forall index: nat :: index in connections.Keys ==> index < i_width);
+      assert Seq.HasNoDuplicates(mp.inputs);
+      reveal Seq.HasNoDuplicates();
+      var np_connections := (map i_index | i_index in connections :: mp.inputs[i_index] := mp.outputs[connections[i_index]]);
+      assert np_connections.Values == GetConnectedOutputs(mp) by {
+        forall onp | onp in np_connections.Values
+          ensures onp in GetConnectedOutputs(mp)
+        {
+          var o_index: nat :| o_index < |mp.outputs| && mp.outputs[o_index] == onp;
+          assert o_index in connections.Values;
+        }
+        forall onp | onp in GetConnectedOutputs(mp)
+          ensures onp in np_connections.Values
+        {
+          var o_index: nat :| o_index < |mp.outputs| && mp.outputs[o_index] == onp;
+          assert o_index in connections.Values;
+          var i_index :| i_index in connections && connections[i_index] == o_index;
+          assert onp == mp.outputs[connections[i_index]];
+          assert np_connections[mp.inputs[i_index]] == onp;
+        }
+      }
+      np_connections
+    }
+
+    function FIFirstPass(mp: ScufMap, fi: FI): (fi_first_pass: FI)
+      requires Valid()
+      requires mp.Valid()
+      requires MPConnectionConsistent(mp, this)
+      requires
+        var new_mp := ConnectScufMap(mp, this);
+        FIValid(fi, new_mp.inputs, new_mp.state)
+      ensures fi_first_pass.state == fi.state
+      ensures FIValid(fi_first_pass, mp.inputs, mp.state)
+    {
+      var output_width := |mp.outputs|;
+      var fake_output := seq(output_width, (index: nat) requires index < output_width => false);
+      var new_mp := ConnectScufMap(mp, this);
+      var sni_first_pass := new_mp.fi2si(fi);
+      var si_first_pass := SI(NIO2I(sni_first_pass.inputs, fake_output), sni_first_pass.state);
+      var fi_first_pass := mp.si2fi(si_first_pass);
+      assert fi_first_pass.state == fi.state by {
+        MapToSeqToMap(mp.state, fi.state);
+      }
+      fi_first_pass
+    }
+
+    function FISecondPass(mp: ScufMap, uf: UpdateFunction, fi: FI): (fi_second_pass: FI)
+      requires Valid()
+      requires mp.Valid()
+      requires uf.Valid()
+      requires MPConnectionConsistent(mp, this)
+      requires UFConnectionConsistent(uf, this)
+      requires ScufMapUpdateFunctionConsistent(mp, uf)
+      requires
+        var new_mp := ConnectScufMap(mp, this);
+        FIValid(fi, new_mp.inputs, new_mp.state)
+      ensures FIValid(fi_second_pass, mp.inputs, mp.state)
+    {
+      var new_mp := ConnectScufMap(mp, this);
+      var sni_first_pass := new_mp.fi2si(fi);
+      var fake_outputs := seq(uf.output_width, (index: nat) requires index < uf.output_width => false);
+      var si_first_pass := SI(NIO2I(sni_first_pass.inputs, fake_outputs), sni_first_pass.state);
+      reveal UpdateFunction.Valid();
+      var so_first_pass := uf.sf(si_first_pass);
+      var si_second_pass := SI(NIO2I(sni_first_pass.inputs, so_first_pass.outputs), sni_first_pass.state);
+      var fi_second_pass := mp.si2fi(si_second_pass);
+      fi_second_pass
+    }
+
+  }
+
+  ghost predicate NoPathInScuf(c: Circuit, s: Scuf, onp: NP, inp: NP)
+    requires c.Valid()
+    requires s.Valid(c)
+    requires NPValid(c, onp)
+  {
+    forall fi: FI :: FIValid(fi, s.mp.inputs, s.mp.state) ==> (
+      assert FICircuitValid(c, fi) by {
+        s.SomewhatValidToRelaxInputs(c);
+        ScufValidFiValidToFICircuitValid(c, s, fi);
+      }
+      var new_fi := FI(fi.inputs - {inp}, fi.state);
+      assert FICircuitValid(c, new_fi) by {
+        reveal FICircuitValid();
+      }
+      Evaluate(c, onp, fi) == Evaluate(c, onp, new_fi)
+    )
+  }
+
+  opaque ghost predicate ScufConnectionConsistent(c: Circuit, s: Scuf, conn: InternalConnection)
+    requires c.Valid()
+    requires s.Valid(c)
+    requires conn.Valid()
+  {
+    reveal InternalConnection.Valid();
+    && (conn.i_width == s.uf.input_width)
+    && (conn.o_width == s.uf.output_width)
+    && (forall i_index, o_index :: i_index in conn.connections && o_index in conn.connections.Values ==>
+        var inp := s.mp.inputs[i_index];
+        var onp := s.mp.outputs[o_index];
+        s.SomewhatValidToRelaxInputs(c);
+        ScufFOutputsAreValid(c, s);
+        ScufFInputsAreValid(c, s);
+        NoPathInScuf(c, s, onp, inp))
+    && (forall i_index :: i_index in conn.connections ==> s.mp.inputs[i_index] !in c.PortSource)
+  }
+
+  predicate UFConnectionConsistent(uf: UpdateFunction, conn: InternalConnection)
+  {
+    && (conn.i_width == uf.input_width)
+    && (conn.o_width == uf.output_width)
+  }
+
+  predicate MPConnectionConsistent(mp: ScufMap, conn: InternalConnection)
+  {
+    && (conn.i_width == |mp.inputs|)
+    && (conn.o_width == |mp.outputs|)
+  }
+
+  lemma ScufConsistentUFMPConsistent(c: Circuit, s: Scuf, conn: InternalConnection)
+    requires c.Valid()
+    requires s.Valid(c)
+    requires conn.Valid()
+    requires ScufConnectionConsistent(c, s, conn)
+    ensures UFConnectionConsistent(s.uf, conn)
+    ensures MPConnectionConsistent(s.mp, conn)
+  {
+    reveal ScufConnectionConsistent();
+  }
+
+  opaque ghost predicate InserterConnectionConsistent(z: ScufInserter, conn: InternalConnection)
+    requires z.Valid()
+    requires conn.Valid()
+  {
+    reveal ScufInserter.Valid();
+    && UFConnectionConsistent(z.uf, conn)
+    && forall c: Circuit :: c.Valid() ==> (
+      z.ValidForCircuit(c);
+      var (new_c, s) := z.fn(c);
+      assert new_c.Valid() && s.Valid(new_c) by {
+        reveal SimpleInsertion();
+      }
+      ScufConnectionConsistent(new_c, s, conn)
+    )
+  }
+
+  function ConnectUpdateFunction(uf: UpdateFunction, conn: InternalConnection): (new_uf: UpdateFunction)
+    requires uf.Valid()
+    requires conn.Valid()
+    requires UFConnectionConsistent(uf, conn)
+    ensures new_uf.Valid()
+  {
+    reveal UpdateFunction.Valid();
+    UpdateFunction(
+      conn.ni_width,
+      uf.output_width,
+      uf.state_width,
+      (sni: SI) requires |sni.inputs| == conn.ni_width && |sni.state| == uf.state_width =>
+        var fake_bo := seq(uf.output_width, index requires 0 <= index < uf.output_width => false);
+        var fake_bi := conn.NIO2I(sni.inputs, fake_bo);
+        var fake_si := SI(fake_bi, sni.state);
+        var fake_so := uf.sf(fake_si);
+        var bi := conn.NIO2I(sni.inputs, fake_so.outputs);
+        var si := SI(bi, sni.state);
+        var so := uf.sf(si);
+        so
+    )
+  }
+
+
+  lemma SelfConnectFirstPassMFLookup(s: Scuf, conn: InternalConnection, np: NP, fi: FI)
+    requires s.MapValid()
+    requires conn.Valid()
+    requires MPConnectionConsistent(s.mp, conn)
+    requires UFConnectionConsistent(s.uf, conn)
+    requires np in conn.GetConnectedOutputs(s.mp)
+    requires
+      var new_s := ConnectScuf(s, conn);
+      FIValid(fi, new_s.mp.inputs, new_s.mp.state)
+    ensures
+      var new_s := ConnectScuf(s, conn);
+      var fi_first_pass := conn.FIFirstPass(s.mp, fi);
+      assert FIValid(fi_first_pass, s.mp.inputs, s.mp.state);
+      reveal Seq.ToSet();
+      MFLookup(s, fi_first_pass, np) == MFLookup(new_s, fi, np)
+  {
+  }
+
+  lemma SelfConnectSecondPassMFLookup(s: Scuf, conn: InternalConnection, np: NP, fi: FI)
+    requires s.MapValid()
+    requires conn.Valid()
+    requires MPConnectionConsistent(s.mp, conn)
+    requires UFConnectionConsistent(s.uf, conn)
+    requires np in s.mp.outputs || np in StateINPs(s.mp.state)
+    requires
+      var new_s := ConnectScuf(s, conn);
+      FIValid(fi, new_s.mp.inputs, new_s.mp.state)
+    ensures
+      var new_s := ConnectScuf(s, conn);
+      var fi_second_pass := conn.FISecondPass(s.mp, s.uf, fi);
+      assert FIValid(fi_second_pass, s.mp.inputs, s.mp.state);
+      reveal Seq.ToSet();
+      MFLookup(s, fi_second_pass, np) == MFLookup(new_s, fi, np)
+  {
+  }
+
+  function ConnectScufMap(mp: ScufMap, conn: InternalConnection): (new_mp: ScufMap)
+    requires mp.Valid()
+    requires conn.Valid()
+    requires MPConnectionConsistent(mp, conn)
+    ensures new_mp.Valid()
+    ensures
+      var connection := conn.GetConnection(mp);
+      && Seq.ToSet(new_mp.inputs) + connection.Keys == Seq.ToSet(mp.inputs)
+      && Seq.ToSet(new_mp.inputs) == Seq.ToSet(mp.inputs) - connection.Keys
+  {
+    var new_mp := ScufMap(
+      conn.I2NI(mp.inputs),
+      mp.outputs,
+      mp.state);
+    conn.I2NIProperties(mp.inputs);
+    new_mp
+  }
+
+  function ConnectScuf(s: Scuf, conn: InternalConnection): (new_scuf: Scuf)
+    requires s.MapValid()
+    requires conn.Valid()
+    requires UFConnectionConsistent(s.uf, conn)
+    ensures new_scuf.MapValid()
+  {
+    var new_s := Scuf(s.sc, ConnectScufMap(s.mp, conn), ConnectUpdateFunction(s.uf, conn));
+    assert new_s.MapValid() by {
+      assert new_s.mp.Valid();
+      assert new_s.mp.InSc(new_s.sc) by {
+        reveal NPsInSc();
+      }
+      assert new_s.uf.Valid();
+      assert ScufMapUpdateFunctionConsistent(new_s.mp, new_s.uf);
+    }
+    new_s
+  }
+
+  lemma ConnectCircuitConnOutputsConstant(c: Circuit, s: Scuf, conn: InternalConnection)
+    requires c.Valid()
+    requires s.Valid(c)
+    requires conn.Valid()
+    requires ScufConnectionConsistent(c, s, conn)
+    ensures
+      var connection := conn.GetConnection(s.mp);
+      var new_c := ConnectCircuit(c, connection);
+      ConnOutputs(c, s.sc) == ConnOutputs(new_c, s.sc)
+  {
+  }
+
+  lemma ConnectCircuitAllInputsDecreases(c: Circuit, s: Scuf, conn: InternalConnection)
+    requires c.Valid()
+    requires s.Valid(c)
+    requires conn.Valid()
+    requires ScufConnectionConsistent(c, s, conn)
+    ensures
+      var connection := conn.GetConnection(s.mp);
+      var new_c := ConnectCircuit(c, connection);
+      && AllInputs(c, s.sc) == AllInputs(new_c, s.sc) + connection.Keys
+      && AllInputs(c, s.sc) - connection.Keys == AllInputs(new_c, s.sc)
+  {
+  }
+
+  function ConnectCircuitScufImpl(c: Circuit, s: Scuf, conn: InternalConnection): (r: (Circuit, Scuf))
+    requires c.Valid()
+    requires s.Valid(c)
+    requires conn.Valid()
+    requires ScufConnectionConsistent(c, s, conn)
+    ensures
+      var (new_c, new_s) := r;
+      && new_c.Valid()
+      && s.MapValid()
+      && ScValid(c, s.sc)
+      && s.SomewhatValidRelaxInputs(c)
+      && new_s.MapValid()
+      && new_s.SomewhatValid(new_c)
+  {
+    reveal ScufConnectionConsistent();
+    var connection := conn.GetConnection(s.mp);
+    conn.GetConnectionProperties(c, s);
+    var new_c := ConnectCircuit(c, connection);
+    var new_s := ConnectScuf(s, conn);
+    assert new_s.SomewhatValid(new_c) by {
+      assert s.Valid(c);
+      reveal Scuf.SomewhatValid();
+      assert ScValid(new_c, new_s.sc) by {
+        reveal ScValid();
+      }
+      assert (AllONPs(new_c, new_s.sc) >= Seq.ToSet(new_s.mp.outputs) >= ConnOutputs(new_c, new_s.sc)) by {
+        reveal AllONPs();
+        reveal Seq.ToSet();
+        reveal ConnOutputs();
+        ConnectCircuitConnOutputsConstant(c, s, conn);
+        assert ConnOutputs(new_c, new_s.sc) == ConnOutputs(c, s.sc);
+      }
+      assert (Seq.ToSet(new_s.mp.inputs) == AllInputs(new_c, new_s.sc)) by {
+        assert Seq.ToSet(s.mp.inputs) == AllInputs(c, new_s.sc);
+        ConnectCircuitAllInputsDecreases(c, s, conn);
+        assert Seq.ToSet(new_s.mp.inputs) == Seq.ToSet(s.mp.inputs) - connection.Keys;
+        assert AllInputs(new_c, new_s.sc) == AllInputs(c, s.sc) - connection.Keys;
+      }
+      assert (Seq.ToSet(new_s.mp.state) == AllSeq(new_c, new_s.sc)) by {
+        reveal AllSeq();
+      }
+    }
+    assert s.ValidRelaxInputs(new_c) by {
+      assert ScValid(new_c, s.sc) by {
+        assert ScValid(c, s.sc);
+        reveal ScValid();
+        assert new_c.NodeKind == c.NodeKind;
+      }
+      assert s.SomewhatValidRelaxInputs(new_c) by {
+      }
+      assert s.EvaluatesCorrectly(new_c) by {
+      }
+    }
+    (new_c, new_s)
+  }
+
+  function ConnectCircuitScuf(c: Circuit, s: Scuf, conn: InternalConnection): (r: (Circuit, Scuf))
+    requires c.Valid()
+    requires s.Valid(c)
+    requires conn.Valid()
+    requires ScufConnectionConsistent(c, s, conn)
+    ensures
+      var (new_c, new_s) := r;
+      && new_c.Valid()
+      && new_s.Valid(new_c)
+      && s.ValidRelaxInputs(new_c)
+  {
+    reveal ScufConnectionConsistent();
+    var (new_c, new_s) := ConnectCircuitScufImpl(c, s,conn);
+    assert new_s.Valid(new_c) by {
+      assert ScValid(new_c, s.sc) by {
+        assert ScValid(c, s.sc);
+        reveal ScValid();
+        assert new_c.NodeKind == c.NodeKind;
+      }
+      assert s.SomewhatValid(new_c) by {
+      }
+      assert s.EvaluatesCorrectly(new_c) by {
+      }
+    }
+    (new_c, new_s)
+  }
+
+}
