SelfConnectEval.dfy
@@ -1,0 +1,224 @@
+module ConnectEval {
+
+  import opened Circ
+  import opened Scuf
+  import opened SelfConnect
+  import opened MapFunction
+  import opened Eval
+  import opened Subcircuit
+
+  ghost predicate ConnectRequirements(c: Circuit, s: Scuf, conn: InternalConnection, fi: FI)
+  {
+    && c.Valid()
+    && s.Valid(c)
+    && conn.Valid()
+    && ScufConnectionConsistent(c, s, conn)
+    && assert conn.i_width == |s.mp.inputs| by {
+      reveal ScufConnectionConsistent();
+    }
+    && FIValid(fi, conn.I2NI(s.mp.inputs), s.mp.state)
+    //&& var (new_c, new_s) := ConnectCircuitScufImpl(c, s, conn);
+    //&& FICircuitValid(new_c, fi)
+  }
+
+  //lemma EvaluateONPInnerFirstPass(c: Circuit, s: Scuf, conn: InternalConnection, fi: FI, path: seq<NP>)
+  //  requires
+  //    var (new_c, new_s) := ConnectCircuitScufImpl(c, s, conn);
+  //    && EvaluateONPInnerRequirements(new_c, path, fi)
+  //    && PathInSubcircuit(path, s.sc)
+  //  ensures
+  //    var (new_c, new_s) := ConnectCircuitScufImpl(c, s, conn);
+  //    var fi_first_pass := conn.FIFirstPass(s.mp, fi);
+  //    && var np := Seq.Last(path);
+  //    && (EvaluateONPInner(new_c, path, fi) == EvaluateONPInner(new_c, path, fi_first_pass))
+  //  decreases
+  //    var (new_c, new_s) := ConnectCircuitScufImpl(c, s, conn);
+  //    |NodesNotInPath(new_c, path)|, 6
+  //{
+  //}
+  lemma EvaluateSelfConnectOldONP(c: Circuit, s: Scuf, conn: InternalConnection, np: NP, fi: FI)
+    //
+    // Here we need to prove that when we take a circuit and connect some of the input points to
+    // other nodes it doesn't effect the evaluation.
+    // This is because at the input points the evaluation is terminated.
+    //
+    requires c.Valid()
+    requires s.Valid(c)
+    requires conn.Valid()
+    requires ScufConnectionConsistent(c, s, conn)
+    requires FIValid(fi, s.mp.inputs, s.mp.state)
+    requires NPValid(c, np)
+    requires np in s.mp.outputs || np in StateINPs(s.mp.state)
+    ensures
+      var (new_c, new_s) := ConnectCircuitScufImpl(c, s, conn);
+      && FICircuitValid(new_c, fi)
+      && (Evaluate(new_c, np, fi) == Evaluate(c, np, fi))
+
+  lemma EvaluateSelfConnectFirstPassONP(c: Circuit, s: Scuf, conn: InternalConnection, np: NP, fi: FI)
+    //
+    // Here we prove that if when we evaluate one of the outputs that we have connected to an input,
+    // the result of the evaluation is not effected is we remove the connected inputs from the
+    // termination points.
+    // This is true because we enforce that there are not paths from the connected outputs to the connected
+    // inputs.
+    //
+    requires ConnectRequirements(c, s, conn, fi)
+    requires
+      var (new_c, new_s) := ConnectCircuitScufImpl(c, s, conn);
+      && NPValid(new_c, np)
+      && (np in conn.GetConnectedOutputs(s.mp))
+    ensures
+      var (new_c, new_s) := ConnectCircuitScufImpl(c, s, conn);
+      var fi_first_pass := conn.FIFirstPass(s.mp, fi);
+      && FICircuitValid(new_c, fi)
+      && FICircuitValid(new_c, fi_first_pass)
+      && (Evaluate(new_c, np, fi_first_pass) == Evaluate(new_c, np, fi))
+
+  lemma EvaluateSelfConnectSecondPassONP(c: Circuit, s: Scuf, conn: InternalConnection, np: NP, fi: FI)
+    //
+    // Here we prove that if when we evaluate an output using inputs created by fi_second_pass
+    // it is equivalent to using the fi inputs.
+    //
+    // The different between these two inputs is that `fi` does not contain elements from the connected
+    // inputs so to prove this we need to show that the values in fi_second_pass match match the values
+    // that are calculated using fi.
+    //
+    requires ConnectRequirements(c, s, conn, fi)
+    requires
+      var (new_c, new_s) := ConnectCircuitScufImpl(c, s, conn);
+      && NPValid(new_c, np)
+      && (np in new_s.mp.outputs || np in StateINPs(new_s.mp.state))
+    ensures
+      var (new_c, new_s) := ConnectCircuitScufImpl(c, s, conn);
+      var fi_second_pass := conn.FISecondPass(s.mp, s.uf, fi);
+      && FICircuitValid(new_c, fi)
+      && FICircuitValid(new_c, fi_second_pass)
+      && (Evaluate(new_c, np, fi_second_pass) == Evaluate(new_c, np, fi))
+
+  //lemma EvaluateSelfConnectFirstPass(c: Circuit, s: Scuf, conn: InternalConnection, np: NP, fi: FI)
+  //  //
+  //  // Here we prove that our evaluation of the circuit matches the UF model.
+  //  // We know that the old scuf is still valid but we still need to prove that the updated
+  //  // update function matches this conserved behavior.
+  //  //
+  //  requires ConnectRequirements(c, s, conn, fi)
+  //  requires
+  //    var (new_c, new_s) := ConnectCircuitScufImpl(c, s, conn);
+  //    && NPValid(new_c, np)
+  //    && (np in conn.GetConnectedOutputs(s.mp))
+  //    && s.SomewhatValidRelaxInputs(new_c)
+  //    && new_s.SomewhatValidRelaxInputs(new_c)
+  //  ensures
+  //    var (new_c, new_s) := ConnectCircuitScufImpl(c, s, conn);
+  //    var fi_first_pass := conn.FIFirstPass(s.mp, fi);
+  //    && FICircuitValid(new_c, fi)
+  //    && FICircuitValid(new_c, fi_first_pass)
+  //    && assert np in new_s.mp.outputs by {
+  //      reveal Seq.ToSet();
+  //    }
+  //    && (Evaluate(new_c, np, fi) == EvalOk(MFLookup(new_s, fi, np)))
+  //{
+  //  var (new_c, new_s) := ConnectCircuitScufImpl(c, s, conn);
+  //  var fi_first_pass := conn.FIFirstPass(s.mp, fi);
+
+  //  assert FICircuitValid(new_c, fi ) by {
+  //    assert FIValid(fi, new_s.mp.inputs, new_s.mp.state);
+  //    ScufValidFiValidToFICircuitValid(new_c, new_s, fi);
+  //    reveal FICircuitValid();
+  //  }
+
+  //  assert FICircuitValid(new_c, fi_first_pass) by {
+  //    assert FIValid(fi_first_pass, s.mp.inputs, s.mp.state);
+  //    ScufValidFiValidToFICircuitValid(new_c, s, fi_first_pass);
+  //    reveal FICircuitValid();
+  //  }
+
+  //  calc {
+  //    Evaluate(new_c, np, fi);
+  //    {
+  //      EvaluateSelfConnectFirstPassONP(c, s, conn, np, fi);
+  //    }
+  //    Evaluate(new_c, np, fi_first_pass);
+  //    {
+  //      EvaluateSelfConnectOldONP(c, s, conn, np, fi_first_pass);
+  //    }
+  //    Evaluate(c, np, fi_first_pass);
+  //    {
+  //      assert s.Valid(c);
+  //      reveal Seq.ToSet();
+  //      reveal Scuf.EvaluatesCorrectly();
+  //    }
+  //    EvalOk(MFLookup(s, fi_first_pass, np));
+  //    {
+  //      SelfConnectFirstPassMFLookup(s, conn, np, fi);
+  //    }
+  //    EvalOk(MFLookup(new_s, fi, np));
+  //  }
+  //}
+
+  lemma EvaluateSelfConnect(c: Circuit, s: Scuf, conn: InternalConnection, np: NP, fi: FI)
+    requires ConnectRequirements(c, s, conn, fi)
+    requires
+      var (new_c, new_s) := ConnectCircuitScufImpl(c, s, conn);
+      && (np in new_s.mp.outputs || np in StateINPs(new_s.mp.state))
+      && FIValid(fi, new_s.mp.inputs, new_s.mp.state)
+      && s.SomewhatValidRelaxInputs(new_c)
+      && new_s.SomewhatValidRelaxInputs(new_c)
+    ensures
+      var (new_c, new_s) := ConnectCircuitScufImpl(c, s, conn);
+      && FICircuitValid(new_c, fi)
+      && NPValid(new_c, np)
+      && (Evaluate(new_c, np, fi) == EvalOk(MFLookup(new_s, fi, np)))
+  {
+    var (new_c, new_s) := ConnectCircuitScufImpl(c, s, conn);
+    var connection := conn.GetConnection(s.mp);
+    var fi_first_pass := conn.FIFirstPass(s.mp, fi);
+    var fi_second_pass := conn.FISecondPass(s.mp, s.uf, fi);
+
+    assert NPValid(c, np) && NPValid(new_c, np) by {
+      assert np in s.mp.outputs || np in StateINPs(s.mp.state);
+      ScufFInputsAreValid(c, s);
+      ScufFOutputsAreValid(c, s);
+      ScufFInputsAreValid(new_c, s);
+      ScufFOutputsAreValid(new_c, s);
+    }
+
+    assert FICircuitValid(new_c, fi ) by {
+      assert FIValid(fi, new_s.mp.inputs, new_s.mp.state);
+      ScufValidFiValidToFICircuitValid(new_c, new_s, fi);
+      reveal FICircuitValid();
+    }
+    assert FICircuitValid(new_c, fi_second_pass) by {
+      assert FIValid(fi_second_pass, s.mp.inputs, s.mp.state);
+      ScufValidFiValidToFICircuitValid(new_c, s, fi_second_pass);
+    }
+    assert FICircuitValid(c, fi_second_pass) by {
+      assert FIValid(fi_second_pass, s.mp.inputs, s.mp.state);
+      ScufValidFiValidToFICircuitValid(c, s, fi_second_pass);
+    }
+
+    calc {
+      Evaluate(new_c, np, fi);
+      {
+        EvaluateSelfConnectSecondPassONP(c, s, conn, np, fi);
+      }
+      Evaluate(new_c, np, fi_second_pass);
+      {
+        EvaluateSelfConnectOldONP(c, s, conn, np, fi_second_pass);
+      }
+      Evaluate(c, np, fi_second_pass);
+      {
+        assert s.Valid(c);
+        reveal Seq.ToSet();
+        reveal Scuf.EvaluatesCorrectly();
+      }
+      EvalOk(MFLookup(s, fi_second_pass, np));
+      {
+        SelfConnectSecondPassMFLookup(s, conn, np, fi);
+      }
+      EvalOk(MFLookup(new_s, fi, np));
+    }
+
+  }
+
+}
